MLIR/Examples/SemanticsTests.lean
@@ -17,7 +17,7 @@ def Test.name: Test → String
 def Test.run (t: Test): String :=
   let (@Test.mk α σ ε δ S _ r) := t
   let t := semanticsRegion 99 r []
-  let t := interp_ub! t
+  let t := interpUB'! t
   let t := interpSSA' t SSAEnv.empty
   let t := t.interp' S.handle
   let t := t.interp ControlFlowOp.handleLogged
